verif/btrees/verif_findindex.v
@@ -63,13 +63,13 @@ Proof.
   destruct n as [ptr0 le isLeaf First Last pn].
   pose (n:= btnode val ptr0 le isLeaf First Last pn). fold n.
   rewrite unfold_btnode_rep. unfold n. Intros ent_end.
-  forward.                      (* t'7=node->numKeys *)
+  forward.                      (* t'4=node->numKeys *)
   simpl in H. destruct isLeaf; try inv H.
   gather_SEP 0 1 2 3. replace_SEP 0 (btnode_rep n).
   { rewrite unfold_btnode_rep with (n:=n). entailer!. Exists ent_end. entailer!. }
 
   forward_if (PROP ( )
-     LOCAL (temp _t'7 (Vint (Int.repr (Z.of_nat (numKeys (btnode val ptr0 le false First Last pn)))));
+     LOCAL (temp _t'4 (Vint (Int.repr (Z.of_nat (numKeys (btnode val ptr0 le false First Last pn)))));
      temp _i (Vint (Int.repr 0)); temp _node (getval (btnode val ptr0 le false First Last pn));
      temp _key (key_repr key))  SEP (btnode_rep n)).
   - forward.                    (* skip *)
@@ -86,62 +86,70 @@ Proof.
     destruct ptr0; try inv H0.  (* keyval isn't possible in an intern node *)
     rewrite unfold_btnode_rep. unfold n. simpl. Intros ent_end0.
     forward.                    (* t'6=node->entries[0]->key *)
-    forward_if.
-    + forward.                  (* return *)
-      entailer!. unfold findChildIndex'. simpl.
-      rewrite key_unsigned_repr in H. rewrite key_unsigned_repr in H.
-      apply Fcore_Zaux.Zlt_bool_true in H. rewrite H. simpl. auto.
-      rewrite unfold_btnode_rep with (n:=(btnode val ptr0 (cons val (keychild val k n0) le') false First Last pn)).
-      Exists ent_end0. entailer!.
-    + forward.                  (* skip *)
-      forward.                  (* i=0 *)
-      gather_SEP 0 1 2 3 4 5. replace_SEP 0 (btnode_rep n).
-      { rewrite unfold_btnode_rep with (n:=n). unfold n.
-        entailer!. Exists ent_end0. entailer!. } deadvars!.
+    gather_SEP 0 1 2 3 4 5. replace_SEP 0 (btnode_rep n).
+    { rewrite unfold_btnode_rep with (n:=n). unfold n.
+      entailer!. Exists ent_end0. entailer!. } deadvars!.      
       
-{ forward_loop (EX i:Z, PROP(i<=Z.of_nat(numKeys n) -1) LOCAL(temp _i (Vint(Int.repr i)); temp _node pn; temp _key (key_repr key)) SEP(btnode_rep n))
-                   break:(EX i:Z, PROP(i=Z.of_nat(numKeys n) -1) LOCAL(temp _i (Vint(Int.repr i)); temp _node pn; temp _key (key_repr key)) SEP(btnode_rep n)).
+{ forward_loop (EX i:nat, PROP((i <= numKeys n)%nat; findChildIndex' le key im = findChildIndex' (skipn_le le i) key (prev_index_nat i)) LOCAL(temp _i (Vint(Int.repr (Z.of_nat i))); temp _node pn; temp _key (key_repr key)) SEP(btnode_rep n))
+                   break:(EX i:nat, PROP() LOCAL(temp _i (Vint(Int.repr (Z.of_nat i))); temp _node pn; temp _key (key_repr key)) SEP(btnode_rep n)).
 
-  - Exists 0. entailer!.
-    destruct (Pos.of_succ_nat (numKeys_le le')).
-    apply Pos2Z.is_nonneg. apply Pos2Z.is_nonneg. omega.
-    
-    (* rewrite key_unsigned_repr in H. rewrite key_unsigned_repr in H. *)
-    (* apply Z.ge_le in H. *)
-    (* apply Fcore_Zaux.Zlt_bool_false in H. rewrite H. *)
-    (* replace 0 with (idx_to_Z (ip O)). *)
-    (* apply FCI_increase. auto. *)
-  - Intros i.
-    rewrite unfold_btnode_rep. unfold n. Intros ent_end1.
+  - Exists O.
+    entailer!. omega.
+  - Intros i. clear ent_end ent_end0.
+    rewrite unfold_btnode_rep. unfold n. Intros ent_end.
     forward.                    (* t'5=node->numKeys *)
     gather_SEP 0 1 2 3 4 5 6. replace_SEP 0 (btnode_rep n).
-    { rewrite unfold_btnode_rep with (n:=n). unfold n. entailer!. Exists ent_end1. entailer!. } 
-    assert((numKeys (btnode val ptr0 (cons val (keychild val k n0) le') false First Last pn)) = S (numKeys_le le')). { simpl. auto. }
-    rewrite H3.
+    { rewrite unfold_btnode_rep with (n:=n). unfold n. entailer!. Exists ent_end. entailer!. }
     forward_if.
-    + entailer!.
-      clear -H1. unfold node_wf in H1. simpl in H1.
-      rewrite Zpos_P_of_succ_nat.
-      rewrite Int.signed_repr.      
-      rewrite Int.signed_repr by rep_omega. rep_omega.
-      rep_omega.
-    + forward.                  (* rest of the loop *)
-      admit.                    (* TODO *)
+    + forward.                  (* skip *)
+      clear ent_end. rewrite unfold_btnode_rep. unfold n. Intros ent_end.
+      assert(HRANGE: (i < numKeys_le le)%nat).
+      { rewrite Zpos_P_of_succ_nat in H3.
+        rewrite Int.signed_repr in H3. rewrite Int.signed_repr in H3.
+        rewrite HLE. simpl. omega.
+        unfold node_wf in H1. simpl in H1. rep_omega.
+        unfold n in H. unfold node_wf in H1. simpl in H, H1. rep_omega. }
+      assert(NTHENTRY: exists ei, nth_entry_le i le = Some ei).
+      { apply nth_entry_le_in_range. auto. }
+      destruct NTHENTRY as [ei NTHENTRY].
+      assert(ZNTH: nth_entry_le i le = Some ei) by auto.
+      eapply Znth_to_list with (endle:=ent_end) in ZNTH. 
+      
+      forward.                  (* t'2=node->entries+i->key *)
+      { entailer!. split. omega. unfold node_wf in H1. simpl in H1. simpl in HRANGE.
+        rewrite Fanout_eq in H1. omega. }
+      { entailer!. simpl in ZNTH. rewrite ZNTH. destruct ei; simpl; auto. }
+      rewrite HLE in ZNTH. rewrite ZNTH.
+      forward_if.
+      * forward.                (* return i-1 *)
+        { entailer!. admit. }
+        entailer!.
+        { replace (if k_ key <? k_ k then im else findChildIndex' le' key (ip 0)) with
+              (findChildIndex' (cons val (keychild val k n0) le') key im) by (simpl; auto).
+          rewrite H2.
+          f_equal. f_equal. admit. }
+        rewrite unfold_btnode_rep with (n:= btnode val ptr0 (cons val (keychild val k n0) le') false First Last pn).
+        Exists ent_end. cancel.
+      * forward.                (* skip *)
+        forward.                (* i++ *)
+        { entailer!. admit. }
+        Exists (S i). entailer!. split.
+        { rewrite H2. admit. }
+        rewrite Zpos_P_of_succ_nat. rewrite <- Z.add_1_r. auto.
+        rewrite unfold_btnode_rep with (n:=n). unfold n. Exists ent_end.
+        cancel.
     + forward.                  (* break *)
-      Exists (Z.of_nat (numKeys n) -1). entailer!.      
-      admit.                    (* TODO *)
-  - Intros i.                   (* after the loop *)
-    rewrite unfold_btnode_rep. unfold n. Intros ent_end1.
-    forward.                    (* t'2=node->numKeys *)
-    forward.                    (* return *)
-    + entailer!. rewrite Zpos_P_of_succ_nat. unfold node_wf in H1. simpl in H1. clear -H1.
-      rewrite Int.signed_repr. rewrite Int.signed_repr.
-      rewrite Zsuccminusone. rep_omega. rep_omega. rep_omega.
-    + 
-      (* prove that numKeys-1 is FCI *)
-      admit. }
-Admitted.
-
+      admit.
+  - Intros i. clear ent_end ent_end0.
+    rewrite unfold_btnode_rep. unfold n. Intros ent_end.
+    forward.                     (* t'1=node->numKeys *)
+    forward.                     (* return t'1-1 *)
+    + entailer!. admit.
+    + entailer!.
+      * admit.
+      * rewrite unfold_btnode_rep with (n:=btnode val ptr0 (cons val (keychild val k n0) le') false First Last pn).
+        Exists ent_end. cancel.
+Admitted.    
 
 Lemma body_findRecordIndex: semax_body Vprog Gprog f_findRecordIndex findRecordIndex_spec.
 Proof.
